

MTH 553: Lecture # 13

Cliff Sun

February 18, 2026

Lecture Span

- HWE in \mathbb{R}^2 and \mathbb{R}^3

HWE on \mathbb{R}^2 and \mathbb{R}^3

Consider $h \in C(\mathbb{R}^n)$ for $n \leq 2$. Then define

$$M_h(x, r) = \int_{S^{n-1}} h(x + r\xi) \frac{d\xi}{\omega_n} \quad (1)$$

Where $d\xi$ is a surface area element in S^{n-1} and $\omega_n = |S^{n-1}|$ is the area of S^{n-1} . We note that $\xi \in S^{n-1}$ is a unit sphere and is a unit vector. Moreover, M_h is the mean of the average value of the h over a sphere of radius $|r|$. For $n = 2$, we have that ω_2 is 2π . Then

$$M_h(x, r) = \frac{1}{2\pi} \int_0^{2\pi} h(x + r\xi) d\theta \quad (2)$$

Where $\xi = (\cos \theta, \sin \theta)$. For $n = 3$, then $\omega_3 = 4\pi$.

Observe

1. $M(h, -r) = M(h, r)$
2. If $h \in C^k$, then $M_h \in C^k$.

Lemma 0.1. (Darboux) For $h \in C^2$ and $r \neq 0$, then

$$\left(\partial_r^2 + \frac{n-1}{r} \partial_r \right) M_h = M_{\nabla^2 h}(x, r) \quad (3)$$

In other words, the laplacian of the mean is the mean of the laplacian.

Proof. When $n = 2$. Consider $e^{i\theta}$ on the unit circle. For $r > 0$: LHS:

$$\frac{1}{2\pi} \int_0^{2\pi} (g_{rr} + \frac{1}{r} g(-r)) d\theta \quad (4)$$

Note that $g(re^{i\theta}) = h(x + re^{i\theta})$. We just took r derivatives.

$$= \frac{1}{2\pi} \int_0^{2\pi} (g_{rr} + \frac{1}{r} g_r + \frac{1}{r^2} g_{\theta\theta}) d\theta \quad (5)$$

Since g is periodic and therefore a closed integral is zero. But this is the Laplacian of g

$$\int_0^{2\pi} \nabla^2 g(re^{i\theta}) \frac{d\theta}{2\pi} \quad (6)$$

$$\iff \int_0^{2\pi} \nabla^2 h(x + re^{i\theta}) \frac{d\theta}{2\pi} \quad (7)$$

$$= M_{\nabla^2 h}(x, r) \quad (8)$$

□

Proof. When $n \geq 2$. Then LHS is

$$= \left(\partial_r + \frac{n-1}{r} \right) \int_{\partial S^n} g_r \frac{d\xi}{\omega_n} \quad (9)$$

Here, the boundary of the ball in S^n is the sphere in S^{n-1} . Then integrate over a sphere of radius r (NOT 1)

$$= \left(\partial_r + \frac{n-1}{r} \right) \int_{\partial B^n(r)} \nabla g(y) \cdot \vec{v} \frac{dS(y)}{r^{n-1}} \quad (10)$$

Then, do a change of variables $y = r\xi$ and $dS(y) = r^{n-1}d\xi$, \vec{v} is the outward normal vector on $\partial B^n(r)$ at $r\xi$. Note that $\nabla g(y) \cdot v = g_r$. Now, we use the divergence theorem

$$\frac{1}{\omega_n} \left(\partial_r + \frac{n-1}{r} \right) \left[\frac{1}{r^{n-1}} \int_{B^n(r)} \nabla \cdot \nabla g(y) dy \right] \quad (11)$$

$$= \frac{1}{\omega_n} \left(\partial_r + \frac{n-1}{r} \right) \left[\frac{1}{r^{n-1}} \int_{B^n(r)} \nabla^2 g(y) dy \right] \quad (12)$$

In spherical coordinates, this is the same as:

$$= \frac{1}{\omega_n} \left(\partial_r + \frac{n-1}{r} \right) \left[\frac{1}{r^{n-1}} \int_0^r \int_{S^{n-1}} \nabla^2 g(\rho, \xi) d\xi \rho^{n-1} d\rho \right] \quad (13)$$

Next, by integrating in spherical coordinates, firstly the following equation is true:

$$\left(\partial_r + \frac{n-1}{r} \right) \frac{1}{r^{n-1}} = 0 \quad (14)$$

Next,

$$\frac{1}{\omega_n} \frac{1}{r^{n-1}} \int_{S^{n-1}} \nabla^2 g(r, \xi) d\xi r^{n-1} \quad (15)$$

$$= \frac{1}{\omega_n} \int_{S^{n-1}} \nabla^2 g(r, \xi) d\xi = M_{\nabla^2 h}(x, r) \quad (16)$$

□

Homogenous wave equation in \mathbb{R}^3

$$\begin{aligned} u_{tt} - c^2 \nabla^2 u &= 0 \\ u(x, 0) &= g(x) \in C^3 \\ u_t(x, 0) &= h(x) \in C^3 \end{aligned}$$

For $x \in \mathbb{R}^3$.

Kirchoff's Formula

$u \in C^2(\mathbb{R}^3 \times [0, \infty))$. Solves HWE in \mathbb{R}^3 if

$$u(x, t) = \partial_t \left(t \int_{S^2} g(x + ct\xi) \frac{d\xi}{4\pi} \right) + t \int_{S^2} h(x + ct\xi) \frac{d\xi}{4\pi} \quad (17)$$

The first term is the displacement response. The second term is the response to the initial impulse.

Proof. (\implies) For all fixed x , $rM_u(x, r)$ satisfies the 1-d wave equation as a function of r and t .

Proof. For $r \neq 0$, we have that $\partial_t^2 (rM_u(x, r)) = rM_{u_{tt}}(x, r)$ □

$$= c^2 r M_{\nabla^2 u}(x, r) \quad (18)$$

$$= c^2 r \left(\partial_r^2 + \frac{2}{r} \partial_r \right) M_u(x, r) \quad (19)$$

by the wave equation and Darboux. Here, we assumed that u satisfied the wave equation.

$$= c^2 \partial_r^2 (r M_u(x, r)) \quad (20)$$

By the product rule. Now, by d'Alembert,

$$r M_u(x, r) = \frac{1}{2} ((r + ct) M_g(x, r + ct) + (r - ct) M_g(x, r - ct)) + \frac{1}{2c} \int_{r-ct}^{r+ct} \rho M_h(x, \rho) d\rho \quad (21)$$

$$= \frac{1}{2} \{ (ct + r) M_g(x, ct + r) + -(ct - r) M_g(x, ct - r) \} + \frac{1}{2c} \int_{ct-r}^{ct+r} \rho M_h(x, \rho) d\rho \quad (22)$$

Here, since by oddness,

$$\int_{r-ct}^{ct-r} \rho M_h(x, \rho) d\rho = 0$$

Now, fix t and divide by r and let $r \rightarrow 0$. Therefore, $M_u \rightarrow u$ and $ct \pm r \rightarrow ct$. Therefore, we get:

$$u(x, r) = \partial_\tau (\tau M_g(x, \tau)) \Big|_{\tau=ct} + \frac{1}{c} \cdot ct M_h(x, ct) \quad (23)$$

Then, use Kirchoff's. □